lib/Camlcoq.ml
@@ -273,8 +273,8 @@ let coqint_of_camlint : int32 -> Integers.Int.int = Z.of_uint32
 let camlint64_of_coqint : Integers.Int64.int -> int64 = Z.to_int64
 let coqint_of_camlint64 : int64 -> Integers.Int64.int = Z.of_uint64
    (* interpret the int64 as unsigned so that result Z is in range for int *)
-let camlint64_of_ptrofs : Integers.Ptrofs.int -> int64 =
-  fun x -> Z.to_int64 (Integers.Ptrofs.signed x)
+(*let camlint64_of_ptrofs : Integers.Ptrofs.int -> int64 =
+  fun x -> Z.to_int64 (Integers.Ptrofs.signed x)*)
 let camlint_of_coqnat : Datatypes.nat -> int = Nat.to_int
 
 (* Atoms (positive integers representing strings) *)
