common/Determinism.v
@@ -52,18 +52,18 @@ Module Deterministic (P:Policy).
 
 CoInductive world: Type :=
   World (io: string -> list eventval -> option (eventval * world))
-        (vload: memory_chunk -> ident -> ptrofs -> option (eventval * world))
-        (vstore: memory_chunk -> ident -> ptrofs -> eventval -> option world).
+        (vload: memory_chunk -> ident -> int64 -> option (eventval * world))
+        (vstore: memory_chunk -> ident -> int64 -> eventval -> option world).
 
 Definition nextworld_io (w: world) (evname: string) (evargs: list eventval) :
                      option (eventval * world) :=
   match w with World io vl vs => io evname evargs end.
 
-Definition nextworld_vload (w: world) (chunk: memory_chunk) (id: ident) (ofs: ptrofs) :
+Definition nextworld_vload (w: world) (chunk: memory_chunk) (id: ident) (ofs: int64) :
                      option (eventval * world) :=
   match w with World io vl vs => vl chunk id ofs end.
 
-Definition nextworld_vstore (w: world) (chunk: memory_chunk) (id: ident) (ofs: ptrofs) (v: eventval):
+Definition nextworld_vstore (w: world) (chunk: memory_chunk) (id: ident) (ofs: int64) (v: eventval):
                      option world :=
   match w with World io vl vs => vs chunk id ofs v end.
 
